Nlp/Syntax.lean
@@ -1,4 +1,5 @@
 import Nlp.Syntax.Tree
+import Nlp.Syntax.TreeLemmas
 import Nlp.Syntax.AnnTree
 
 /-! Constituency syntax data structures. -/
